project/relational_graph_IG_basic_operations.v
@@ -1,0 +1,96 @@
+Require Import String.
+Require Import Coq.Arith.Arith.
+Open Scope string_scope.
+
+Require Import List.
+Require Import Bool.
+Import ListNotations.
+
+Require Import MyProject.project.util.util.
+
+Require Import MyProject.project.relational_graph.
+Require Import MyProject.project.relational_graph_theory.
+
+
+Require Import Coq.Sets.Ensembles.
+Require Import MyProject.project.util.NatSet.
+
+
+
+(* Now start defining the basic IG functions in terms of an RG *)
+  (* {-# MINIMAL empty, isEmpty, match, mkGraph, labNodes #-} *)
+
+
+(* Start defining functionality: *)
+Definition RG_empty : RG nat :=
+    RG_empty.
+
+
+Definition RG_isEmpty (rg : RG nat) : Prop :=
+  RG_isEmpty rg.
+
+
+
+(* Helper for matsh *)
+Definition _eliminate (node : Node) (rg : RG nat) : RG nat.
+Proof.
+  refine {|
+      RG_nodes := Subtract nat (rg.(RG_nodes)) node;
+      RG_edges := fun (n0 n1 : nat) => n0 <> node /\ n1 <> node /\  rg.(RG_edges) n0 n1;
+      RG_valid := _
+  |}.
+  RG_valid_prover_with rg.
+  - unfold not. intros. inversion H2. congruence.
+  - unfold not. intros. inversion H2. congruence.
+Defined.
+
+Definition _getFromsAndTos (node : Node) (rg : RG nat) : Prop * (Ensemble nat * Ensemble nat) :=
+  (rg.(RG_nodes) node, ((fun (from : nat) => rg.(RG_edges) from node), (fun (to : nat) => rg.(RG_edges) node to)))
+.
+
+
+(* (Ensemble nat * Ensemble nat) is not a relation, it is two _independent_ sets of from- and to- neighbors *)
+Definition RG_matsh (node : Node) (rg : RG nat) : (Prop * (Ensemble nat * Ensemble nat)) * RG nat :=
+  (_getFromsAndTos node rg, _eliminate node rg)
+.
+
+
+
+Definition _add (node : Node) (fromsTos : (NatSet.t * NatSet.t)) (rg : RG nat) : RG nat :=
+  match fromsTos with | (froms, tos) =>
+    _extendByContext node froms tos rg
+  end
+.
+
+
+Definition _insNode (node : Node) (rg : RG nat) : RG nat :=
+  _add node (NatSet.empty, NatSet.empty) rg.
+  
+
+Definition _insNodes (nodes : list Node) (rg : RG nat) : RG nat :=
+  fold_right _insNode rg nodes.
+
+
+(* If one of the nodes of the edge does not exist, nothing happens *)
+Definition _insEdge (edge : (Node * Node)) (rg : RG nat) : RG nat.
+Proof.
+  destruct edge as [node0 node1].
+    refine {|
+      RG_nodes := rg.(RG_nodes);
+      RG_edges := fun (n0 n1 : nat) => (n0 = node0 /\ n1 = node1 /\ rg.(RG_nodes) node0 /\ rg.(RG_nodes) node1) \/  rg.(RG_edges) n0 n1;
+      RG_valid := _
+  |}.
+  RG_valid_prover_with rg.
+  - congruence.
+  - congruence.
+Defined.
+
+
+Definition _insEdges (edges : list (Node * Node)) (rg : RG nat) : RG nat :=
+  fold_right _insEdge rg edges.
+
+Definition RG_mkGraph (nodes : list Node) (edges : list (Node * Node)) : RG nat :=
+  _insEdges edges (_insNodes nodes RG_empty).
+ 
+Definition RG_labNodes (rg : RG nat) : Ensemble Node :=
+  rg.(RG_nodes).
