project/util/NatSet.v
@@ -1,0 +1,6 @@
+Require Import FSets.
+
+Definition Node := Nat_as_OT.t.
+
+Module NatSet := FSetList.Make(Nat_as_OT).
+Module NatSetProperties := EqProperties(NatSet).
